add sha224-mb and sha384-mb

code/sha2-vec/Hacl.SHA2.Scalar32.fst
@@ -23,6 +23,29 @@ module SpecVec = Hacl.Spec.SHA2.Vec
 
 [@CInline]
 private
+val sha224_update1: update_vec_t SHA2_224 M32
+let sha224_update1 b hash = update #SHA2_224 #M32 b hash
+
+
+val sha224: hash:lbuffer uint8 28ul -> len:size_t -> b:lbuffer uint8 len ->
+  Stack unit
+  (requires fun h0 -> live h0 b /\ live h0 hash /\ disjoint hash b)
+  (ensures  fun h0 _ h1 -> modifies (loc hash) h0 h1 /\
+    as_seq h1 hash == Spec.hash #SHA2_224 (v len) (as_seq h0 b))
+
+let sha224 h len b =
+  let h0 = ST.get() in
+  let b = ntup1 b in
+  let h = ntup1 h in
+  hash #SHA2_224 #M32 (sha224_update1 <: update_vec_t SHA2_224 M32) h len b;
+  let h1 = ST.get() in
+  Hacl.Spec.SHA2.Equiv.hash_lemma #SHA2_224 #M32 (v len) (as_seq_multi h0 b);
+  let hash0 = tup1 h in
+  assert ((as_seq_multi h1 h).(|0|) == as_seq h1 hash0)
+
+
+[@CInline]
+private
 val sha256_update1: update_vec_t SHA2_256 M32
 let sha256_update1 b hash = update #SHA2_256 #M32 b hash
 
@@ -40,6 +63,29 @@ let sha256 h len b =
   hash #SHA2_256 #M32 (sha256_update1 <: update_vec_t SHA2_256 M32) h len b;
   let h1 = ST.get() in
   Hacl.Spec.SHA2.Equiv.hash_lemma #SHA2_256 #M32 (v len) (as_seq_multi h0 b);
+  let hash0 = tup1 h in
+  assert ((as_seq_multi h1 h).(|0|) == as_seq h1 hash0)
+
+
+[@CInline]
+private
+val sha384_update1: update_vec_t SHA2_384 M32
+let sha384_update1 b hash = update #SHA2_384 #M32 b hash
+
+
+val sha384: hash:lbuffer uint8 48ul -> len:size_t -> b:lbuffer uint8 len ->
+  Stack unit
+  (requires fun h0 -> live h0 b /\ live h0 hash /\ disjoint hash b)
+  (ensures  fun h0 _ h1 -> modifies (loc hash) h0 h1 /\
+    as_seq h1 hash == Spec.hash #SHA2_384 (v len) (as_seq h0 b))
+
+let sha384 h len b =
+  let h0 = ST.get() in
+  let b = ntup1 b in
+  let h = ntup1 h in
+  hash #SHA2_384 #M32 (sha384_update1 <: update_vec_t SHA2_384 M32) h len b;
+  let h1 = ST.get() in
+  Hacl.Spec.SHA2.Equiv.hash_lemma #SHA2_384 #M32 (v len) (as_seq_multi h0 b);
   let hash0 = tup1 h in
   assert ((as_seq_multi h1 h).(|0|) == as_seq h1 hash0)
 
